% This is for chapter 3
\section{The ROC Surface of Modified Extended Neyman Pearson Test}

\subsection{Modified Receiver of Characteristic of MENP test}

The ROC surface of MENP test (M-ROC) depicts the relationship between $P_d$ and $c_1, c_2, ..., c_M$. On one hand, it  illustrates the largest $P_d$ can be achieved under the constraint $\mathbf{P}_{f} \leq \mathbf{c}$, on the other hand, it provides the range of $\mathbf{c}$ for a given $P_d$.
Points $(P_d, c_1, c_2, ..., c_M)$ on M-ROC  surface can be divided into two types: 
\\1. Those with $[c_1, c_2, ..., c_M] \in \alpha^+$. Define this set of points as $M_0$; 
\\2. Those with $[c_1, c_2, ..., c_M] \notin \alpha^+$. Define this set of points as $M_1$. 

Obviously points in $M_0$ can be achieved by MENP (\rmnum{1}) and points in $M_1$ can  be achieved by MENP (\rmnum{2}). Next we consider a property of M-ROC surface.

\noindent \textbf{Property 1}
\noindent \textit{
  \noindent Assume hypotheses given as:
}
\begin{equation}
  \begin{split}
	H_0:\;\;\;\;\;\;&X \sim f_0(x)\\
	H_1:\;\;\;\;\;\;&X \sim f_1(x)\\
	&......\\
	H_M:\;\;\;\;\;\;&X \sim f_M(x)
  \end{split}
\end{equation}
\textit{
  define $g(x) = \frac{\sum_{i=1}^{M}k_if_i(x)}{f_0(x)}$ and let $F_i(x)$ represent the CDF of hypothesis $H_i$ ($i = 1, ..., M$). If $g(x)$ is a monotonically increasing function of $x$ for any non-negative $k_i\;\;(i = 1, ..., M)$ and $F_i(x)$ is monotonically increasing function, then we have:}

  \textit{(1)The region achieved by ENP test with non-negative parameters degenerates to a curve.}

  \textit{(2)For a specific false alarm constraints $P_{f_i} \leq c_i\;\;(i = 1, ..., M)$, the decision rule for MENP test is $x \substack{\bar{H}_0 \\ \geq \\ < \\H_0} x_0$, where $x_0 = \min\{F_1^{-1}(c_1), ..., F_M^{-1}(c_M)\}$.}

  \textit{(3)The expression of $P_d$, $P_{f_1}$, ..., $P_{f_M}$ can be written as}
  \begin{equation}
	\label{equ: chi pd}
	\begin{split}
	  P_d & = F_0(x_0)\\
	  P_{f_1} & = F_1(x_0)\\
	  &......\\
	  P_{f_M} & = F_M(x_0)
	\end{split}
  \end{equation}

  \noindent \textbf{PROOF}
  According to the definition, $M_0$ is the region achieved by ENP test with $k_i \geq 0 (i=1, ..., M)$. The ENP decision rule is
  \begin{equation}
	\label{1127a}
	\frac{\sum_{i=1}^{M}k_if_i(x)}{f_0(x)} \substack{\bar{H}_0 \\\geq\\< \\H_0}1\,.
  \end{equation}
  From the condition $g(x) = \frac{\sum_{i=1}^{M}k_if_i(x)}{f_0(x)} $, \eqref{1127a} can be written as 
  \begin{equation}
	\label{dec: gx}
	g(x)\substack{\bar{H}_0 \\\geq\\< \\H_0}1
  \end{equation}
  Since $g(x)$ is a monotonically increasing function with $x$, hence $g^{-1}(x)$ exists and \eqref{dec: gx} can be written in form of 
  \begin{equation}
	\label{dec: x0}
	x\substack{\bar{H}_0 \\\geq\\< \\H_0}x_0\,,
  \end{equation}
  where $x_0 = g^{-1}(1)$.
  Under decision rule \eqref{dec: x0}, the expression of $P_d$, $P_{f_1}$, ..., $P_{f_M}$ is: 
  \begin{equation}
	\begin{split}
	  \label{equ: pd under x0}
	  P_d &= \text{Pr}(X \leq x_0 | H_0) = F_0(x_0)\\
	  P_{f_1} &= \text{Pr}(X \leq x_0 | H_1) = F_1(x_0)\\
	  &......\\
	  P_{f_M} &= \text{Pr}(X \leq x_0 | H_M) = F_M(x_0)
	\end{split}
  \end{equation}
  where $F_0$, $F_1$, ..., $F_M$ are the CDFs of $X$ under $H_0$, $H_1$, ..., $H_M$. From \eqref{equ: pd under x0}, $P_{f_1}$ determines $x_0$ that in turn determines $P_{f_2}$, ..., $P_{f_M}$, $P_d$. Hence for a given $P_{f_1}$, there is only one corresponding $P_{f_i} (i= 1, ..., M)$. Hence the ROC surface with $k_i \geq 0 (i = 1, ..., M)$ degenerates to a curve in this case.

  Furthermore, \eqref{dec: x0}  implies for an ENP decision rule with non-negative parameters, there exists an $x_0$ such that the ENP decision rule can be written in form of 
  \begin{equation}
	\label{1125 dec: x0}
	x\substack{\bar{H}_0 \\\geq\\< \\H_0}x_0\,.
  \end{equation}

  Next we consider the optical decision rule $\delta^\ast$ of
  \begin{equation}
	\begin{split}
	  \max\;\;\;\; &P_d\\
	  \text{s.t.}\;\;\;\;&\mathbf{P}_f \leq \mathbf{c}\,,
	\end{split}
  \end{equation}
  where $\mathbf{c} \in (0, 1)$.
  From \textbf{Lemma 1} we know $\delta^\ast$ is an ENP test with non-negative parameters, hence according to our previous discussion there exists an $x_0$ such that $\delta^\ast$ can be written in form of 
  \begin{equation}
	\label{1124a1}
	x\substack{\bar{H}_0 \\\geq\\< \\H_0}x_0\,,
  \end{equation}
  and the expression of $P_d$ and $\mathbf{P}_f$ are given in \eqref{equ: pd under x0}. 
  In the following, we will determine the value of $x_0$. 
  As $P_d$ is an increasing function with respect to $x_0$, in order to acquire the maximum $P_d$ we need to achieve the largest $x_0$ while keeping 
  \begin{equation}
	P_{f_i} \leq c_i\;\;\;\;(i = 1, 2, ..., M)\,.
  \end{equation}
  Substitute \eqref{equ: pd under x0} into above equation, we have
  \begin{equation}
	F_i(x_0) \leq c_i \;\;\;\;(i=1, 2, ..., M)\,.
  \end{equation}
  \begin{equation}
	\label{1125a1}
	\therefore\;\;\;\; x_0 \leq F^{-1}_{i}(c_i) \;\;\;\;(i=1, 2, ..., M)\,.
  \end{equation}
  \eqref{1125a1} can be fulfilled only if $x_0$ is 
  smaller or equal to the minimum of $F^{-1}_{i}(c_i)$ ($i=1, 2, ..., M$). This implies the largest $x_0$ can be achieved is $\min\{F_1^{-1}(c_1), F_2^{-1}(c_2), ..., F_M^{-1}(c_M)\}$, i.e.
  \begin{equation}
	\label{1127a2}
	x_0 = \min(F_1^{-1}(c_1), F_2^{-1}(c_2), ..., F_M^{-1}(c_M))\,.
  \end{equation}
  And by  using decision rule \eqref{1125 dec: x0}, we have
  \begin{equation}
	\begin{split}
	  \label{equ: pd under x00}
	  P_d &=  F_0(x_0)\\
	  P_{f_1} &=  F_1(x_0)\\
	  &......\\
	  P_{f_M} &= F_M(x_0)\,.
	\end{split}
  \end{equation}
%==================================================================================================
  \typeout{}
  \input{3/gaussian}

%==================================================================================================
  \typeout{}
  \input{3/chisquare}
